some tweaks to the interface

pulse/pulse2rust/src/ocaml/RustBindings.ml
@@ -6,7 +6,7 @@ module Rust = struct
   (* external add_2 : i64 -> string = "rust_add_2"
 
   external dflt : i64 option -> string = "rust_dflt" *)
-  external fn_to_rust : Pulse2Rust_Rust_Syntax.fn -> string = "rust_fn_to_syn_string"
+  external file_to_rust : Pulse2Rust_Rust_Syntax.file -> string = "rust_file_to_syn_string"
   external fn_to_string : Pulse2Rust_Rust_Syntax.fn -> string = "rust_fn_to_string"
   external expr_to_string : Pulse2Rust_Rust_Syntax.expr -> string = "rust_expr_to_string"
   external typ_to_string : Pulse2Rust_Rust_Syntax.typ -> string = "rust_typ_to_string"
@@ -14,7 +14,7 @@ end
 (* let add_2 (x:i64) = Rust.add_2 x
 let dflt (x:i64 option) = Rust.dflt x *)
 
-let fn_to_rust f = Rust.fn_to_rust f
+let file_to_rust f = Rust.file_to_rust f
 let fn_to_string f = Rust.fn_to_string f
 let expr_to_string e = Rust.expr_to_string e
 let typ_to_string t = Rust.typ_to_string t
